Derived_co_Pairs.v
@@ -70,14 +70,14 @@ Module Make(Import M: Memory.T).
 
 (** COPAIRS **)
 
- Definition cppermut {X Y} : term (X + Y) (Y + X) := copair coproj2 coproj1.
+ Definition cppermut {X Y} : term (X + Y) (Y + X) := copair in2 in1.
  Definition rcopair {X Y Z} (f1: term X Y) (f2: term X Z) : term X (Y + Z) := copair f2 f1 o (@cppermut Z Y).
 
  Lemma ss_rcopair_eq: forall A B1 B2 d (f1: term A B1) (f2: term A B2),
- PPG d f2 -> CTC d f1 -> rcopair f1 f2 o coproj1 === f1.
+ PPG d f2 -> CTC d f1 -> rcopair f1 f2 o in1 === f1.
  Proof.
     intros A B1 B2 d f1 f2 H1 H2. unfold rcopair, cppermut. rewrite <- assoc.
-    cut (copair coproj2 coproj1 o coproj1 === (@coproj2 B2 B1)).
+    cut (copair in2 in1 o in1 === (@in2 B2 B1)).
       intro H0. rewrite H0. apply (@ss_lcopair_eq _ _ _ d). exact H1.
     (*1st cut*)
     apply (@swtoss _ _ pure); try edecorate.
@@ -85,20 +85,20 @@ Module Make(Import M: Memory.T).
  Qed.
 
  Lemma sw_rcopair_eq: forall A B1 B2 d (f1: term A B1) (f2: term A B2),
- PPG d f2 -> CTC d f1 -> rcopair f1 f2 o coproj2 ==~ f2.
+ PPG d f2 -> CTC d f1 -> rcopair f1 f2 o in2 ==~ f2.
  Proof.
     intros A B1 B2 d f1 f2 H1 H2. unfold rcopair, cppermut. rewrite <- assoc.
-    cut (copair coproj2 coproj1 o coproj2 === (@coproj1 B2 B1)).
+    cut (copair in2 in1 o in2 === (@in1 B2 B1)).
       intro H0. rewrite H0. apply (@sw_lcopair_eq _ _ _ d); induction d; edecorate.
     (*1st cut*)
     apply (@ss_lcopair_eq _ _ _ pure); edecorate.
  Qed.
 
  Lemma ss_lcopair_u: forall A B1 B2 (f g: term A (B1 + B2)),
- (f o coproj1 ==~ g o coproj1) -> (f o coproj2 === g o coproj2) -> f === g.
+ (f o in1 ==~ g o in1) -> (f o in2 === g o in2) -> f === g.
  Proof.
     intros A B1 B2 f g H1 H2. apply eeffect.
-    cut ((@coproj2 B1 B2) o (@empty B2) === (@empty (B1 + B2))).
+    cut ((@in2 B1 B2) o (@empty B2) === (@empty (B1 + B2))).
       intro H0. rewrite <- H0. setoid_rewrite assoc.
       apply replsubs; [exact H2 | reflexivity].
     (*1st cut*)
@@ -107,10 +107,10 @@ Module Make(Import M: Memory.T).
  Qed.
 
  Lemma ss_rcopair_u: forall A B1 B2 (f g: term A (B1 + B2)),
- (f o coproj1 === g o coproj1) -> (f o coproj2 ==~ g o coproj2) -> f === g.
+ (f o in1 === g o in1) -> (f o in2 ==~ g o in2) -> f === g.
  Proof.
     intros A B1 B2 f g H1 H2. apply eeffect.
-    cut ((@coproj1 B1 B2) o (@empty B1) === (@empty (B1 + B2))).
+    cut ((@in1 B1 B2) o (@empty B1) === (@empty (B1 + B2))).
       intro H0. rewrite <- H0. setoid_rewrite assoc.
       apply replsubs; [exact H1 | reflexivity].
     (*1st cut*)
@@ -119,16 +119,16 @@ Module Make(Import M: Memory.T).
  Qed.
 
  (* additional lemmas about [pbl] and [copair] *)
- Lemma pbl_true: pbl o constant true === coproj1.
+ Lemma pbl_true: pbl o constant true === in1.
  Proof.
-     unfold pbl. unfold constant. rewrite imp6. unfold coproj1.
-     apply imp7. intros. simpl. rewrite x. reflexivity.
+     unfold pbl, constant, in1, bool_to_two. rewrite <- tcomp.
+     apply imp6. intros. rewrite x. reflexivity.
  Qed.
 
- Lemma pbl_false: pbl o constant false === coproj2.
+ Lemma pbl_false: pbl o constant false === in2.
  Proof. 
-    unfold pbl. unfold constant. setoid_rewrite imp6.
-    apply imp7.  now intros [].
+     unfold pbl, constant, in1, bool_to_two. rewrite <- tcomp.
+     apply imp6. intros. rewrite x. reflexivity.
  Qed.
 
  Lemma copair_true: forall k A f g, PPG k f -> PPG k g ->  @copair _ _ A f g o (pbl o constant true) === f.
